Update

project2/reverse/FileUtils.dfy
@@ -58,67 +58,15 @@ method ReadFile(f: FileStream, length: nat32) returns (ok: bool, result: seq<byt
 
     result := buffer[..];
 }
-/* 
-method ReadLine(f: seq<byte>, start: nat) returns (next: nat, line:seq<byte>)
-    requires 0 <= start < |f|
-    requires |f[start..]| > 0
-
-    ensures start < next
-    ensures next <= |f|
-    ensures next == |f| || f[next-1] == '\n' as byte
-    ensures line == f[start..next]
-    ensures forall k :: start <= k < next-1 ==> f[k] != '\n' as byte
-
-    ensures line == head(lines(f[start..]))
-{
-    next := start;
-    line := [];
-    while (next < |f| && f[next] != '\n' as byte)
-        decreases |f| - next
-        invariant start <= next <= |f|
-        invariant line == f[start..next]
-        invariant '\n' as byte !in f[start..next]
-    {
-        line := line + [f[next]];
-        next := next + 1;
-    }
-
-    if (next < |f| && f[next] == '\n' as byte) {
-        line := line + [f[next]];
-        next := next + 1;
-    }
-}
-
-method ReadLines(f: seq<byte>) returns (l: List<seq<byte>>)
-    ensures l == lines(f)
-    //ensures size(lines) == count(f, '\n' as byte) + 1
-{
-    l := Nil;
-    var next := 0;
-    var line := [];
-    while (next != |f|)
-        decreases |f| - next
-        invariant next <= |f|
-        invariant l == lines(f[..next])
-        //invariant size(lines) == count(f[..next], '\n' as byte)
-    {
-        next, line := ReadLine(f, next);
-        concat_unit(l, line);
-        l := append(l, Cons(line, Nil));
-    }
-}
-*/
 
 function method lines(s: seq<byte>): List<seq<byte>>
     ensures |s| > 0 ==> non_empty(lines(s))
-    ensures |concat(lines(s))| <= |s|
 {
   lines_aux(s, [])
 }
 
 function method lines_aux(s: seq<byte>, acum: seq<byte>): List<seq<byte>>
     ensures non_empty(lines_aux(s, acum))
-    ensures |concat(lines_aux(s, acum))| <= |s|
 {
   if s == [] then
     Cons(acum, Nil)
@@ -126,4 +74,21 @@ function method lines_aux(s: seq<byte>, acum: seq<byte>): List<seq<byte>>
     Cons(acum, lines_aux(s[1..], []))
   else
     lines_aux(s[1..], acum + [s[0]])
+}
+
+function method join(l: List<seq<byte>>): seq<byte>
+{
+    match l
+        case Nil => []
+        case Cons(h, T) => if T == Nil then h else h + ['\n' as byte] + join(T)
+}
+
+lemma join_lines_identity(s: seq<byte>)
+    ensures join(lines(s)) == s
+{   
+    if s == [] {
+        
+    } else {
+        
+    }
 }
