project2/grep-kmp/kmp.dfy
@@ -1,0 +1,127 @@
+predicate prefix_suffix<T(==)>(S: seq<T>, k: nat)
+    requires 0 <= k <= |S|
+{
+    S[..k] == S[|S|-k..]
+}
+
+function method match_at<T(==)>(t: seq<T>, p:seq<T>, t_pos:nat): bool
+    requires 0 <= t_pos < |t|
+{
+    p <= t[t_pos..]
+}
+
+lemma smaller_prefix_suffix<T(==)>(P: seq<T>, k:nat, pik:nat)
+    requires 0 <= pik <= k < |P|
+    requires prefix_suffix(P, k)
+    requires prefix_suffix(P[..k], pik)
+    ensures prefix_suffix(P, pik)
+{}
+
+lemma subsubseq<T(==)>(S: seq<T>, i:nat, j:nat)
+    requires 0 <= i <= j <= |S|
+    ensures S[..j][..i] == S[..i]
+{}
+
+predicate lps<T(==)>(S: seq<T>, k:nat)
+    requires 0 <= k <= |S|
+{
+    (|S| == 0 || k < |S|) &&
+    prefix_suffix(S, k) &&
+    forall k' :: k <= k' < |S| ==> !prefix_suffix(S, k')
+}
+
+lemma larger_lps<T(==)>(P:seq<T>, k:nat, q:nat)
+    requires 0 <= k < q < |P|
+    requires lps(P[..q-1], k)
+    requires P[q] == P[k]
+    ensures lps(P[..q], k+1)
+{}
+
+method PrefixFunction<T(==)>(P: seq<T>) returns (pi: array<int>)
+    requires |P| > 1
+
+    ensures pi.Length == |P|
+    ensures forall i :: 0 <= i < |P| ==> 0 <= pi[i] <= i
+    ensures forall i :: 0 <= i < |P| ==> lps(P[..i], pi[i])
+{
+    pi := new int[|P|];
+    pi[0] := 0;
+    var q := 1;
+    var k := 0;
+    while q < pi.Length
+        decreases pi.Length - q
+
+        invariant pi.Length == |P|
+
+        invariant 0 < q <= pi.Length
+        invariant 0 <= k <= q <= |P|
+        invariant forall i :: 0 <= i < q ==> 0 <= pi[i] <= i
+        invariant forall i :: 0 <= i < q ==> lps(P[..i], pi[i])
+    {
+        k := pi[q - 1];
+
+        while k > 0 && P[k] != P[q]
+            decreases k
+            invariant 0 <= k < q
+            invariant k <= q-1
+            invariant forall i :: 0 <= i < q ==> 0 <= pi[i] <= i
+            invariant forall i :: 0 <= i < q ==> lps(P[..i], pi[i])
+            invariant prefix_suffix(P[..q-1], k)
+        {
+            subsubseq(P, k, q-1);
+            smaller_prefix_suffix(P[..q-1], k, pi[k]);
+            k := pi[k - 1];
+        }
+
+        assert prefix_suffix(P[..q-1], k);
+
+        if P[k] == P[q] {
+            larger_lps(P, k, q);
+            k := k + 1;
+        }
+
+        pi[q] := k;
+        q := q + 1;
+    }
+}
+
+method Match<Type(==)>(T: seq<Type>, P: seq<Type>) returns (m: bool, pos:nat)
+    requires |P| > 1
+    requires |T| > 0
+    requires |T| >= |P|
+
+    ensures m ==> 0 <= pos < |T|
+    ensures !m ==> 0 <= pos <= |T|
+    ensures m ==> match_at(T, P, pos)
+    ensures forall k :: 0 <= k < pos ==> !match_at(T, P, k)
+{
+   var lsp := PrefixFunction(P);
+   var i, j := 0, 0;
+    while j < |P| && i < |T|
+        decreases |T| - i
+
+        invariant 0 <= j <= |P|
+        invariant j <= i <= |T|
+        invariant T[i-j..i] == P[..j]
+        invariant forall k :: 0 <= k < i - j ==> !match_at(T, P, k)
+    {
+        while j > 0 && j < |P| && T[i] != P[j]
+            decreases j
+
+            invariant 0 <= j <= |P|
+            invariant j <= i <= |T|
+            //invariant T[i-j..i] == P[..j]
+            //invariant forall k :: 0 <= k < i - j ==> !match_at(T, P, k)   
+        {
+            j := lsp[j-1];
+        }
+
+        if T[i] == P[j] {
+            j := j + 1;
+        }
+
+        i := i + 1;
+    }
+    m := j == |T|;
+    pos := i - j;
+}
