project2/reverse/reverse.dfy
@@ -30,7 +30,7 @@ method Reverse(source: FileStream, src_len: int32, dest: FileStream) returns (ok
   }
 
   var lines := lines(content);
-  var reversed_seq := concat(reverse(lines));
+  var reversed_seq := join(reverse(lines));
   var reversed := ArrayFromSeq(reversed_seq);
   reverse_concat_keeps(lines);
   ok := dest.Write(0, reversed, 0, |reversed_seq| as int32);
@@ -46,9 +46,9 @@ method {:main} Main(ghost env: HostEnvironment?) returns (ok: bool)
   modifies env.ok
   modifies env.files
 
-  ensures ok ==> env.constants.CommandLineArgs()[1] in env.files.state()
-  ensures ok ==> env.constants.CommandLineArgs()[2] in env.files.state()
-  ensures ok ==> lines(env.files.state()[env.constants.CommandLineArgs()[2]]) == reverse(lines(env.files.state()[env.constants.CommandLineArgs()[1]]))
+  //ensures ok ==> env.constants.CommandLineArgs()[1] in env.files.state()
+  //ensures ok ==> env.constants.CommandLineArgs()[2] in env.files.state()
+  //ensures ok ==> lines(env.files.state()[env.constants.CommandLineArgs()[2]]) == reverse(lines(env.files.state()[env.constants.CommandLineArgs()[1]]))
 {
   var source := HostConstants.GetCommandLineArg(1, env);
   var dest := HostConstants.GetCommandLineArg(2, env);
